src/Std/Sat/AIG/If.lean
@@ -96,7 +96,7 @@ def ite (aig : AIG α) (input : IfInput aig w) : RefVecEntry α w :=
 where
   go {w : Nat} (aig : AIG α) (curr : Nat) (hcurr : curr ≤ w) (discr : Ref aig)
       (lhs rhs : RefVec aig w) (s : RefVec aig curr) : RefVecEntry α w :=
-    if hcurr:curr < w then
+    if hcurr : curr < w then
       let input := ⟨discr, lhs.get curr hcurr, rhs.get curr hcurr⟩
       let res := mkIfCached aig input
       let aig := res.aig
