src/Std/Sat/AIG/RefVecOperator/Zip.lean
@@ -88,7 +88,7 @@ where
       (lhs rhs : RefVec aig len) (f : (aig : AIG α) → BinaryInput aig → Entrypoint α)
       [LawfulOperator α BinaryInput f] [chainable : LawfulZipOperator α f] :
       RefVecEntry α len :=
-    if hidx:idx < len then
+    if hidx : idx < len then
       let res := f aig ⟨lhs.get idx hidx, rhs.get idx hidx⟩
       let aig := res.aig
       let newRef := res.ref
